Avoid stack overflow in the extracted code.

src/BBShl.v
@@ -4,6 +4,7 @@ From mathcomp Require Import ssreflect ssrbool ssrnat eqtype seq ssrfun.
 From BitBlasting Require Import QFBV CNF BBCommon BBIte.
 From ssrlib Require Import ZAriths Seqs Tactics.
 From nbits Require Import NBits.
+From Coq Require Import Recdef.
 
 Set Implicit Arguments.
 Unset Strict Implicit.
@@ -16,12 +17,6 @@ Import Prenex Implicits.
 (*   by rewrite /shlB iter_add . *)
 (* Qed . *)
 
-Lemma size_joinlsb T b (bs : seq T) :
-  size (joinlsb b bs) = (size bs) + 1 .
-Proof .
-  by rewrite /= addn1 .
-Qed .
-
 (* Lemma shlB1_size bs : *)
 (*   size (shlB1 bs) = size bs . *)
 (* Proof . *)
@@ -29,20 +24,6 @@ Qed .
 (*   rewrite subn1 addn1 . *)
 (*   reflexivity . *)
 (* Qed . *)
-
-Lemma size_joinlsl T l (ls : seq T) :
-  size (joinlsl l ls) = size ls + 1 .
-Proof .
-  exact : size_joinlsb .
-Qed .
-
-Lemma size_dropmsl ls :
-  size (dropmsl ls) = size ls - 1 .
-Proof .
-  destruct ls => /= .
-  - reflexivity .
-  - by rewrite subn1 -pred_Sn size_belast .
-Qed .
 
 (* Lemma shlB_size n bs : *)
 (*   size (shlB n bs) = size bs . *)
@@ -58,24 +39,77 @@ Qed .
 Definition bit_blast_shl_int1 g ls : generator * cnf * word :=
   (g, [::], dropmsl (joinlsl lit_ff ls)) .
 
-Fixpoint bit_blast_shl_int g ls n : generator * cnf * word :=
+Function bit_blast_shl_int g ls (n : N) {wf N.lt n} : generator * cnf * word :=
   match n with
-  | O => (g, [::], ls)
-  | S m => let '(g_m, cs_m, ls_m) := bit_blast_shl_int g ls m in
-           let '(g1, cs1, ls1) := bit_blast_shl_int1 g_m ls_m in
-           (g1, catrev cs_m cs1, ls1)
+  | N0 => ((g, [::]), ls)
+  | _ =>
+    let '(g_m, cs_m, ls_m) := bit_blast_shl_int g ls (n - 1)%num in
+    let '(g1, cs1, ls1) := bit_blast_shl_int1 g_m ls_m in
+    ((g1, catrev cs_m cs1), ls1)
   end.
+Proof.
+  - move=> _ _ n p Hp. rewrite -Hp. move: (N.le_pred_l n) => Hle.
+    rewrite N.sub_1_r. move/(N.lt_eq_cases (N.pred n) n): Hle. case=> Hn.
+    + assumption.
+    + apply: N.lt_pred_l. move=> Hn0. rewrite Hn0 in Hp. discriminate.
+  - exact: N.lt_wf_0.
+Qed.
 
 Definition mk_env_shl_int1 E g ls : env * generator * cnf * word :=
   (E, g, [::], dropmsl (joinlsl lit_ff ls)) .
 
-Fixpoint mk_env_shl_int E g ls n : env * generator * cnf * word :=
+Function mk_env_shl_int E g ls (n : N) {wf N.lt n} : env * generator * cnf * word :=
   match n with
-  | O => (E, g, [::], ls)
-  | S m => let: (E_m, g_m, cs_m, ls_m) := mk_env_shl_int E g ls m in
-           let: (E', g', cs, ls') := mk_env_shl_int1 E_m g_m ls_m in
-           (E', g', catrev cs_m cs, ls')
+  | N0 => (((E, g), [::]), ls)
+  | _ => let: (E_m, g_m, cs_m, ls_m) := mk_env_shl_int E g ls (n - 1)%num in
+         let: (E', g', cs, ls') := mk_env_shl_int1 E_m g_m ls_m in
+         (((E', g'), catrev cs_m cs), ls')
   end .
+Proof.
+  - move=> _ _ _ n p Hp. rewrite -Hp. move: (N.le_pred_l n) => Hle.
+    rewrite N.sub_1_r. move/(N.lt_eq_cases (N.pred n) n): Hle. case=> Hn.
+    + assumption.
+    + apply: N.lt_pred_l. move=> Hn0. rewrite Hn0 in Hp. discriminate.
+  - exact: N.lt_wf_0.
+Qed.
+
+Lemma bit_blast_shl_int_N0 g ls :
+  bit_blast_shl_int g ls N0 = (g, [::], ls).
+Proof.
+  symmetry. apply: R_bit_blast_shl_int_complete.
+  apply: (R_bit_blast_shl_int_0 _ _ N0). reflexivity.
+Qed.
+
+Lemma bit_blast_shl_int_Npos g ls p g_m cs_m ls_m g' cs1 lrs :
+  bit_blast_shl_int g ls (N.pos p - 1) = (g_m, cs_m, ls_m) ->
+  bit_blast_shl_int1 g_m ls_m = (g', cs1, lrs) ->
+  bit_blast_shl_int g ls (N.pos p) = (g', catrev cs_m cs1, lrs).
+Proof.
+  move=> Hbb Hbb1. move: (Logic.eq_sym Hbb) => {Hbb} Hbb.
+  move: (R_bit_blast_shl_int_correct Hbb) => {Hbb} Hbb.
+  symmetry. apply: R_bit_blast_shl_int_complete.
+  by apply: (R_bit_blast_shl_int_1 _ _ _ _ _ _ _ Hbb _ _ _ _ _ _ _ Hbb1).
+Qed.
+
+Lemma mk_env_shl_int_N0 E g ls :
+  mk_env_shl_int E g ls N0 = (E, g, [::], ls).
+Proof.
+  symmetry. apply: R_mk_env_shl_int_complete.
+  apply: (R_mk_env_shl_int_0 _ _ _ N0). reflexivity.
+Qed.
+
+Lemma mk_env_shl_int_Npos E g ls p E_m g_m cs_m ls_m E' g' cs1 lrs :
+  mk_env_shl_int E g ls (N.pos p - 1) = (E_m, g_m, cs_m, ls_m) ->
+  mk_env_shl_int1 E_m g_m ls_m = (E', g', cs1, lrs) ->
+  mk_env_shl_int E g ls (N.pos p) = (E', g', catrev cs_m cs1, lrs).
+Proof.
+  move=> Hbb Hbb1. move: (Logic.eq_sym Hbb) => {Hbb} Hbb.
+  move: (R_mk_env_shl_int_correct Hbb) => {Hbb} Hbb.
+  symmetry. apply: R_mk_env_shl_int_complete.
+    by apply: (R_mk_env_shl_int_1 _ _ _ _ _ _ _ _ Hbb _ _ _ _ _ _ _ _ _ Hbb1).
+Qed.
+
+
 
 Lemma bit_blast_shl_int1_correct :
   forall g bs E ls g' cs lrs,
@@ -99,24 +133,23 @@ Lemma bit_blast_shl_int_correct :
     interp_cnf E (add_prelude cs) ->
     enc_bits E lrs (shlB n bs).
 Proof.
-  move => g bs .
-  elim .
-  - move => E ls g' cs lrs .
-    rewrite /bit_blast_shl_int /= .
-    case => _ _ <- // .
-  - move => n IH E ls g' cs lrs .
-    rewrite /bit_blast_shl_int (lock interp_cnf) /=
-            -!lock -/bit_blast_shl_int .
-    case Hm: (bit_blast_shl_int g ls n) => [[g_m cs_m] ls_m] .
-    case => _ <- <- .
-    move => Hlsbs Hcsm .
-    rewrite add_prelude_catrev in Hcsm .
-    move : Hcsm => /andP [Hcsm _] .
-    move : (IH _ _ _ _ _ Hm Hlsbs Hcsm) => Hls_mbs .
-    rewrite /shlB1 .
-    apply : enc_bits_dropmsb; first apply: (add_prelude_tt Hcsm) .
-    rewrite enc_bits_joinlsb Hls_mbs (add_prelude_enc_bit_ff Hcsm) // .
-Qed .
+  move => g bs n E ls. eapply bit_blast_shl_int_ind.
+  - clear n. move=> n Hn g' cs lrs. case=> ? ? ?; subst => /=.
+    move=> H _. assumption.
+  - clear n. move=> n [] => //=. move=> p Hn _ IH.
+    move=> g_m cs_m ls_m Hm. move=> g1 cs1 ls1 H1.
+    move=> g' cs lrs. case=> ? ? ?; subst => /=.
+    move=> Henc Hcsm. rewrite add_prelude_catrev in Hcsm.
+    move/andP: Hcsm=> [Hcsm Hcs1]. move: (IH _ _ _ Hm Henc Hcsm) => Hls_mbs.
+    move: (bit_blast_shl_int1_correct H1 Hls_mbs Hcs1).
+    rewrite shlB1_shlB_succ. rewrite -addn1.
+    have ->: ((N.pos p - 1)%num + 1) = nat_of_pos p.
+    { replace 1 with (nat_of_bin 1) by reflexivity.
+      rewrite -nat_of_add_bin. rewrite N.sub_add.
+      - exact: nat_of_bin_pos.
+      - exact: Npos_ge1. }
+    by apply.
+Qed.
 
 Lemma size_bit_blast_shl_int1 g ls g' cs lrs :
   bit_blast_shl_int1 g ls = (g', cs, lrs) ->
@@ -131,52 +164,50 @@ Qed .
 
 Lemma size_bit_blast_shl_int g n ls g' cs lrs :
   bit_blast_shl_int g ls n = (g', cs, lrs) ->
-  size ls = size lrs .
-Proof .
-  rewrite /bit_blast_shl_int /= .
-  elim : n g' cs lrs => [|n IH] g' cs lrs .
-  - by case => _ _ <- .
-  - move: IH; rewrite -/bit_blast_shl_int => IH .
-    dcase (bit_blast_shl_int g ls n) => [[[g_m cs_m] ls_m] Hrec] .
-    case => _ _ <- .
-    move : (IH _ _ _ Hrec) => Hlslsm .
-    rewrite size_dropmsl size_joinlsl .
-    rewrite addn1 subn1 Hlslsm .
-    reflexivity .
-Qed .
+  size ls = size lrs.
+Proof.
+  move: g' cs lrs. eapply bit_blast_shl_int_ind.
+  - clear n. move=> n Hn g' cs lrs [] ? ? ?; subst => /=. reflexivity.
+  - clear n. move=> n [] p Hn //=. move=> _ IH g_m cs_m ls_m Hbb g1 cs1 ls1 Hbb1.
+    move=> g' cs lrs [] ? ? ?; subst => /=. rewrite (IH _ _ _ Hbb).
+    exact: (size_bit_blast_shl_int1 Hbb1).
+Qed.
 
-Fixpoint bit_blast_shl_rec g ls ns i : generator * cnf * word :=
+
+
+Fixpoint bit_blast_shl_rec g ls ns (i : N) : generator * cnf * word :=
   match ns with
   | [::] => (g, [::], ls)
   | ns_hd::ns_tl =>
-    let '(g_tl, cs_tl, ls_tl) := bit_blast_shl_rec g ls ns_tl (2 * i) in
-    let '(g_hd, cs_hd, ls_hd) := bit_blast_shl_int g_tl ls_tl i in
+    let '(g_tl, cs_tl, ls_tl) := bit_blast_shl_rec g ls ns_tl (i * 2)%num in
     if ns_hd == lit_tt then
+      let '(g_hd, cs_hd, ls_hd) := bit_blast_shl_int g_tl ls_tl i in
       (g_hd, catrev cs_tl cs_hd, ls_hd)
     else if ns_hd == lit_ff then
            (g_tl, cs_tl, ls_tl)
          else
+           let '(g_hd, cs_hd, ls_hd) := bit_blast_shl_int g_tl ls_tl i in
            let '(g_ite, cs_ite, ls_ite) := bit_blast_ite g_hd ns_hd ls_hd ls_tl in
            (g_ite, catrev cs_tl (catrev cs_hd cs_ite), ls_ite)
   end .
 
 Definition bit_blast_shl g ls ns : generator * cnf * word :=
-  bit_blast_shl_rec g ls ns 1 .
+  bit_blast_shl_rec g ls ns 1%num.
 
 Lemma bit_blast_shl_rec_correct g bs ns i E ls lns g' cs lrs :
   bit_blast_shl_rec g ls lns i = (g', cs, lrs) ->
   enc_bits E ls bs ->
   enc_bits E lns ns ->
   interp_cnf E (add_prelude cs) ->
-  enc_bits E lrs (shlB (to_nat ns * i) bs) .
-Proof .
+  enc_bits E lrs (shlB (to_nat ns * i) bs).
+Proof.
   move => Hshlrec Hlsbs Hlnsns .
   move : (enc_bits_size Hlnsns) => Hsizelnsns .
   move : lns ns Hsizelnsns i g' cs lrs Hshlrec Hlsbs Hlnsns.
   apply : seq_ind2 => [|lns_hd ns_hd lns_tl ns_tl Hsizelnns IH] i g' cs lrs .
   - by case => _ <- <- .
   - rewrite /= .
-    dcase (bit_blast_shl_rec g ls lns_tl (2*i)) => [[[g_tl cs_tl] ls_tl] Hshlrec] .
+    dcase (bit_blast_shl_rec g ls lns_tl (i * 2)) => [[[g_tl cs_tl] ls_tl] Hshlrec] .
     dcase (bit_blast_shl_int g_tl ls_tl i) => [[[g_hd cs_hd] ls_hd] Hshlint] /= .
     case Hlnshdtt : (lns_hd == lit_tt) .
     + case => _ <- <- Hlsbs Hlnsns Hcnf .
@@ -188,8 +219,8 @@ Proof .
       move/eqP : Hlnshdtt => Hlnshdtt .
       rewrite Hlnshdtt in Hlnsns_hd .
       rewrite (add_prelude_enc_bit_true ns_hd Hcnfcs_tl) in Hlnsns_hd .
-      replace ns_hd with true .
-      rewrite mulnA muln2 /= .
+      rewrite Hlnsns_hd.
+      rewrite nat_of_mul_bin (mulnC i 2%num). rewrite mulnA muln2 /=.
       by rewrite -[(1+ (to_nat ns_tl).*2)*i]/(i + ((to_nat ns_tl).*2)*i) .
     + case Hlnshdff : (lns_hd == lit_ff) .
       * case => _ <- <- Hlsbs Hlnsns Hcnfcs_tl .
@@ -199,7 +230,7 @@ Proof .
         rewrite Hlnshdff in Hlnsns_hd .
         rewrite (add_prelude_enc_bit_is_not_true ns_hd Hcnfcs_tl) in Hlnsns_hd .
         rewrite (negbTE Hlnsns_hd) .
-        by rewrite mulnA muln2 /= .
+          by rewrite nat_of_mul_bin (mulnC i 2%num) mulnA muln2 /=.
       * dcase (bit_blast_ite g_hd lns_hd ls_hd ls_tl) => [[[g_ite cs_ite] ls_ite] Hite] .
         case => _ <- <- Hlsbs Hlnsns Hcnf .
         move : Hcnf; rewrite add_prelude_catrev => /andP [Hcnfcs_tl Hcnfcs_others] .
@@ -212,23 +243,23 @@ Proof .
         rewrite eq_sym in Hlshdtl .
         move : (bit_blast_ite_correct Hlshdtl Hite Hlnsns_hd Hlshdbs Hlstlbs Hcnfcs_ite) .
         destruct ns_hd .
-        + rewrite mulnA muln2 .
+        + rewrite nat_of_mul_bin (mulnC i 2%num) mulnA muln2 .
           by rewrite -[(i+(to_nat ns_tl).*2 * i)]/((true + (to_nat ns_tl).*2)*i) .
-        + rewrite mulnA muln2 .
+        + rewrite nat_of_mul_bin (mulnC i 2%num) mulnA muln2 .
           by rewrite -[(false + (to_nat ns_tl).*2) * i]/((to_nat ns_tl).*2 *i) .
-Qed .
+Qed.
 
 Corollary bit_blast_shl_correct g bs ns E ls lns g' cs lrs :
     bit_blast_shl g ls lns = (g', cs, lrs) ->
     enc_bits E ls bs ->
     enc_bits E lns ns ->
     interp_cnf E (add_prelude cs) ->
-    enc_bits E lrs (shlB (to_nat ns) bs) .
-Proof .
-  move => Hshl Hlsbs Hlnsns Hcnf .
-  rewrite -(muln1 (to_nat ns)) .
-  exact : (bit_blast_shl_rec_correct Hshl Hlsbs Hlnsns Hcnf) .
-Qed .
+    enc_bits E lrs (shlB (to_nat ns) bs).
+Proof.
+  move => Hshl Hlsbs Hlnsns Hcnf.
+  rewrite -(muln1 (to_nat ns)).
+  exact : (bit_blast_shl_rec_correct Hshl Hlsbs Hlnsns Hcnf).
+Qed.
 
 Lemma mk_env_shl_int1_is_bit_blast_shl_int1 E g ls E' g' cs lrs :
     mk_env_shl_int1 E g ls = (E', g', cs, lrs) ->
@@ -240,16 +271,17 @@ Qed .
 
 Lemma mk_env_shl_int_is_bit_blast_shl_int E g ls i E' g' cs lrs :
     mk_env_shl_int E g ls i = (E', g', cs, lrs) ->
-    bit_blast_shl_int g ls i = (g', cs, lrs) .
-Proof .
-  elim: i E' g' cs lrs => [| i IH ] E' g' cs lrs .
-  - rewrite /mk_env_shl_int /bit_blast_shl_int /= .
-    by case => _ <- <- <- .
-  - rewrite /mk_env_shl_int /= -/mk_env_shl_int .
-    dcase (mk_env_shl_int E g ls i) => [[[[E_m g_m] cs_m] ls_m] Henv] .
-    rewrite (IH _ _ _ _ Henv) .
-    by case => _ <- <- <- .
-Qed .
+    bit_blast_shl_int g ls i = (g', cs, lrs).
+Proof.
+  move: E' g' cs lrs. eapply mk_env_shl_int_ind.
+  - clear i. move=> i Hi E' g' cs lrs [] ? ? ? ?; subst => /=.
+    symmetry. apply: R_bit_blast_shl_int_complete.
+    apply: (R_bit_blast_shl_int_0 _ _ 0). reflexivity.
+  - clear i. move=> i [] p Hn //=. move=> _ IH E_m g_m cs_m ls_m Henv.
+    move=> E1 g1 cs1 ls1 Henv1. move=> E' g' cs lrs [] ? ? ? ?; subst => /=.
+    move: (mk_env_shl_int1_is_bit_blast_shl_int1 Henv1) => Hbb1.
+    move: (IH _ _ _ _ Henv) => Hbb. exact: (bit_blast_shl_int_Npos Hbb Hbb1).
+Qed.
 
 Lemma size_mk_env_shl_int1 E g ls E' g' cs lrs :
   mk_env_shl_int1 E g ls = (E', g', cs, lrs) ->
@@ -264,31 +296,29 @@ Qed .
 
 Lemma size_mk_env_shl_int E g n ls E' g' cs lrs :
   mk_env_shl_int E g ls n = (E', g', cs, lrs) ->
-  size ls = size lrs .
-Proof .
-  rewrite /mk_env_shl_int /= .
-  elim : n E' g' cs ls lrs => [|n IH] E' g' cs ls lrs .
-  - by case => _ _ _ <- .
-  - move: IH; rewrite -/mk_env_shl_int => IH .
-    dcase (mk_env_shl_int E g ls n) => [[[[E_m g_m] cs_m] ls_m] Hrec] .
-    case => _ _ _ <- .
-    move : (IH _ _ _ _ _ Hrec) => Hlslsm .
-    rewrite size_dropmsl size_joinlsl .
-    rewrite addn1 subn1 Hlslsm .
-    reflexivity .
-Qed .
+  size ls = size lrs.
+Proof.
+  move: E' g' cs lrs. eapply mk_env_shl_int_ind.
+  - clear n. move=> n Hn E' g' cs lrs [] ? ? ? ?; subst => /=. reflexivity.
+  - clear n. move=> n [] p Hn //=. move=> _ IH E_m g_m cs_m ls_m Hbb.
+    move=> E1 g1 cs1 ls1 Hbb1. move=> E' g' cs lrs [] ? ? ? ?; subst => /=.
+    rewrite (IH _ _ _ _ Hbb). exact: (size_mk_env_shl_int1 Hbb1).
+Qed.
 
-Fixpoint mk_env_shl_rec E g ls ns i : env * generator * cnf * word :=
+
+
+Fixpoint mk_env_shl_rec E g ls ns (i : N) : env * generator * cnf * word :=
   match ns with
   | [::] => (E, g, [::], ls)
   | ns_hd::ns_tl =>
-    let '(E_tl, g_tl, cs_tl, ls_tl) := mk_env_shl_rec E g ls ns_tl (2 * i) in
-    let '(E_hd, g_hd, cs_hd, ls_hd) := mk_env_shl_int E_tl g_tl ls_tl i in
+    let '(E_tl, g_tl, cs_tl, ls_tl) := mk_env_shl_rec E g ls ns_tl (i * 2) in
     if ns_hd == lit_tt then
+      let '(E_hd, g_hd, cs_hd, ls_hd) := mk_env_shl_int E_tl g_tl ls_tl i in
       (E_hd, g_hd, catrev cs_tl cs_hd, ls_hd)
     else if ns_hd == lit_ff then
            (E_tl, g_tl, cs_tl, ls_tl)
          else
+           let '(E_hd, g_hd, cs_hd, ls_hd) := mk_env_shl_int E_tl g_tl ls_tl i in
            let '(E_ite, g_ite, cs_ite, ls_ite) := mk_env_ite E_hd g_hd ns_hd ls_hd ls_tl in
            (E_ite, g_ite, catrev cs_tl (catrev cs_hd cs_ite), ls_ite)
   end .
@@ -304,7 +334,7 @@ Proof .
   - rewrite /mk_env_shl_rec /= -/mk_env_shl_rec .
     by case => _ <- <- <- .
   - rewrite /mk_env_shl_rec /= -/mk_env_shl_rec .
-    dcase (mk_env_shl_rec E g ls ns_tl (2*i)) => [[[[E_tl g_tl] cs_tl] ls_tl] Hrec] .
+    dcase (mk_env_shl_rec E g ls ns_tl (i*2)) => [[[[E_tl g_tl] cs_tl] ls_tl] Hrec] .
     rewrite (IH _ _ _ _ _ Hrec) .
     dcase (mk_env_shl_int E_tl g_tl ls_tl i) => [[[[E_hd g_hd] cs_hd] ls_hd] Hint] .
     rewrite (mk_env_shl_int_is_bit_blast_shl_int Hint) .
@@ -324,15 +354,17 @@ Qed .
 
 Lemma mk_env_shl_int_newer_gen E g ls n E' g' cs lrs :
     mk_env_shl_int E g ls n = (E', g', cs, lrs) ->
-    (g <=? g')%positive .
-Proof .
-  elim : n E' g' cs lrs => [ | n IH] E' g' cs lrs .
-  - rewrite /mk_env_shl_int /=; by t_auto_newer .
-  - rewrite /mk_env_shl_int /= -/mk_env_shl_int .
-    dcase (mk_env_shl_int E g ls n) => [[[[E_m g_m] cs_m] ls_m] Hint] .
-    move : (IH _ _ _ _ Hint) => Hind .
-    t_auto_newer .
-Qed .
+    (g <=? g')%positive.
+Proof.
+  move: E' g' cs lrs. eapply mk_env_shl_int_ind.
+  - clear n. move=> n Hn E' g' cs lrs [] ? ? ? ?; subst => /=.
+    exact: Pos.leb_refl.
+  - clear n. move=> n [] p Hn //=. move=> _ IH E_m g_m cs_m ls_m Henv.
+    move=> E1 g1 cs1 ls1 Henv1. move=> E' g' cs lrs [] ? ? ? ?; subst => /=.
+    move : (IH _ _ _ _ Henv) => {IH Henv} Hind.
+    rewrite /mk_env_shl_int1 in Henv1. case: Henv1 => ? ? ? ?; subst.
+    assumption.
+Qed.
 
 Lemma mk_env_shl_rec_newer_gen E g ls ns i E' g' cs lrs :
     mk_env_shl_rec E g ls ns i = (E', g', cs, lrs) ->
@@ -341,7 +373,7 @@ Proof .
   elim : ns E' g' cs lrs i => [|ns_hd ns_tl IH] E' g' cs lrs i .
   - rewrite /mk_env_shl_rec /=; by t_auto_newer .
   - rewrite /mk_env_shl_rec /= -/mk_env_shl_rec .
-    dcase (mk_env_shl_rec E g ls ns_tl (2*i)) => [[[[E_tl g_tl] cs_tl] ls_tl] Hrec] .
+    dcase (mk_env_shl_rec E g ls ns_tl (i*2)) => [[[[E_tl g_tl] cs_tl] ls_tl] Hrec] .
     move : (IH _ _ _ _ _ Hrec) => Hggtl .
     dcase (mk_env_shl_int E_tl g_tl ls_tl i) => [[[[E_hd g_hd] cs_hd] ls_hd] Hint] .
     move : (mk_env_shl_int_newer_gen Hint) => Hgtlghd .
@@ -368,20 +400,20 @@ Lemma mk_env_shl_int_newer_res E g n E' g' ls cs lrs :
   newer_than_lits g' lrs .
 Proof .
   move => Htt Hls .
-  elim : n E' g' cs lrs => [|n IH] E' g' cs lrs .
-  - rewrite /mk_env_shl_int /=; by t_auto_newer .
-  - rewrite /mk_env_shl_int /= -/mk_env_shl_int .
-    dcase (mk_env_shl_int E g ls n) => [[[[E_m g_m] cs_m] ls_m] Hint] .
-    case => _ <- _ <- .
-    move : (IH _ _ _ _ Hint) => Hlsm .
-    move : (mk_env_shl_int_newer_gen Hint) => Hggm .
-    move : (newer_than_lit_le_newer Htt Hggm) => Hgmtt .
-    generalize Hgmtt .
-    rewrite newer_than_lit_tt_ff => Hgmff .
-    move : (newer_than_lits_joinlsl Hgmff Hlsm) => Hgmjoinlsl .
-    move : (newer_than_lits_splitmsl Hgmtt Hgmjoinlsl) => /andP [Hsplit1 _] .
-    by rewrite /dropmsl .
-Qed .
+  move: E' g' cs lrs. eapply mk_env_shl_int_ind.
+  - clear n. move=> n Hn E' g' cs lrs [] ? ? ? ?; subst => /=.
+    assumption.
+  - clear n. move=> n [] p Hn //=. move=> _ IH E_m g_m cs_m ls_m Henv.
+    move=> E1 g1 cs1 ls1 [] ? ? ? ?; subst. move=> E' g' cs lrs [] ? ? ? ?; subst.
+    move: (IH _ _ _ _ Henv) => Hlsm.
+    move : (mk_env_shl_int_newer_gen Henv) => {Henv} Hggm.
+    move : (newer_than_lit_le_newer Htt Hggm) => Hgmtt.
+    generalize Hgmtt.
+    rewrite newer_than_lit_tt_ff => Hgmff.
+    move : (newer_than_lits_joinlsl Hgmff Hlsm) => Hgmjoinlsl.
+    move : (newer_than_lits_splitmsl Hgmtt Hgmjoinlsl) => /andP [Hsplit1 _].
+    by rewrite /dropmsl.
+Qed.
 
 Lemma mk_env_shl_rec_newer_res E g i E' g' ls ns cs lrs :
   newer_than_lit g lit_tt ->
@@ -394,7 +426,7 @@ Proof .
   - rewrite /mk_env_shl_rec /=; by t_auto_newer .
   - rewrite /mk_env_shl_rec /= -/mk_env_shl_rec .
     move : Hgns; rewrite newer_than_lits_cons => /andP [Hgnshd Hgnstl] .
-    dcase (mk_env_shl_rec E g ls ns_tl (2*i)) => [[[[E_tl g_tl] cs_tl] ls_tl] Hrec] .
+    dcase (mk_env_shl_rec E g ls ns_tl (i*2)) => [[[[E_tl g_tl] cs_tl] ls_tl] Hrec] .
     move : (IH _ _ _ _ _ Hgnstl Hrec) => Hgtllstl .
     move : (mk_env_shl_rec_newer_gen Hrec) => Hggtl .
     dcase (mk_env_shl_int E_tl g_tl ls_tl i) => [[[[E_hd g_hd] cs_hd] ls_hd] Hint] .
@@ -420,13 +452,12 @@ Lemma mk_env_shl_int_newer_cnf E g ls n E' g' cs lr :
     newer_than_lits g ls ->
     newer_than_cnf g' cs .
 Proof .
-  elim : n E' g' cs lr => [|n IH] E' g' cs lr .
-  - rewrite /mk_env_shl_int /=; by case => _ <- <- _ _ .
-  - rewrite /mk_env_shl_int /= -/mk_env_shl_int .
-    dcase (mk_env_shl_int E g ls n) => [[[[E_m g_m] cs_m] ls_m] Hint] .
-    case => _ <- <- _ Hgls .
-    move : (IH _ _ _ _ Hint Hgls) => Hgmcsm .
-    by rewrite newer_than_cnf_catrev Hgmcsm /= .
+  move: E' g' cs lr. eapply mk_env_shl_int_ind.
+  - clear n. move=> n Hn E' g' cs lrs [] ? ? ? ?; subst => /=. done.
+  - clear n. move=> n [] p Hn //=. move=> _ IH E_m g_m cs_m ls_m Henv.
+    move=> E1 g1 cs1 ls1 [] ? ? ? ?; subst. move=> E' g' cs lrs [] ? ? ? ?; subst.
+    move=> Hgls. move : (IH _ _ _ _ Henv Hgls) => Hgmcsm.
+    by rewrite newer_than_cnf_catrev Hgmcsm /=.
 Qed .
 
 Lemma mk_env_shl_rec_newer_cnf E g ls ns i E' g' cs lr :
@@ -438,7 +469,7 @@ Proof .
   elim : ns E' g' cs lr i => [|ns_hd ns_tl IH] E' g' cs lr i .
   - rewrite /mk_env_shl_rec /=; by case => _ <- <- _ .
   - rewrite /mk_env_shl_rec /= -/mk_env_shl_rec .
-    dcase (mk_env_shl_rec E g ls ns_tl (2*i)) => [[[[E_tl g_tl] cs_tl] ls_tl] Hrec] .
+    dcase (mk_env_shl_rec E g ls ns_tl (i*2)) => [[[[E_tl g_tl] cs_tl] ls_tl] Hrec] .
     dcase (mk_env_shl_int E_tl g_tl ls_tl i) => [[[[E_hd g_hd] cs_hd] ls_hd] Hint] .
     dcase (mk_env_ite E_hd g_hd ns_hd ls_hd ls_tl) => [[[[E_ite g_ite] cs_ite] ls_ite] Hite] .
     move => Htemp Hgtt Hgls /andP [Hgnshd Hgnstl] .
@@ -474,15 +505,14 @@ Qed .
 
 Lemma mk_env_shl_int_preserve E g ls n E' g' cs lrs :
     mk_env_shl_int E g ls n = (E', g', cs, lrs) ->
-    env_preserve E E' g .
-Proof .
-  elim : n E' g' cs lrs => [| n IH] E' g' cs lrs .
-  - rewrite /mk_env_shl_int /=; by case => <- _ _ _ .
-  - rewrite /mk_env_shl_int /= -/mk_env_shl_int .
-    dcase (mk_env_shl_int E g ls n) => [[[[E_m g_m] cs_m] ls_m] Hint] .
-    case => <- _ _ _ .
-    by apply : (IH _ _ _ _ Hint) .
-Qed .
+    env_preserve E E' g.
+Proof.
+  move: E' g' cs lrs. eapply mk_env_shl_int_ind.
+  - clear n. move=> n Hn E' g' cs lrs [] ? ? ? ?; subst => /=. done.
+  - clear n. move=> n [] p Hn //=. move=> _ IH E_m g_m cs_m ls_m Henv.
+    move=> E1 g1 cs1 ls1 [] ? ? ? ?; subst. move=> E' g' cs lrs [] ? ? ? ?; subst.
+    exact: (IH _ _ _ _ Henv).
+Qed.
 
 Lemma mk_env_shl_rec_preserve E g ls ns i E' g' cs lrs :
   mk_env_shl_rec E g ls ns i = (E', g', cs, lrs) ->
@@ -491,7 +521,7 @@ Proof .
   elim : ns E' g' cs lrs i => [| ns_hd ns_tl IH] E' g' cs lrs i .
   - rewrite /mk_env_shl_rec /=; by case => <- _ _ _ .
   - rewrite /mk_env_shl_rec /= -/mk_env_shl_rec .
-    dcase (mk_env_shl_rec E g ls ns_tl (2*i)) => [[[[E_tl g_tl] cs_tl] ls_tl] Hrec] .
+    dcase (mk_env_shl_rec E g ls ns_tl (i*2)) => [[[[E_tl g_tl] cs_tl] ls_tl] Hrec] .
     dcase (mk_env_shl_int E_tl g_tl ls_tl i) => [[[[E_hd g_hd] cs_hd] ls_hd] Hint] .
     dcase (mk_env_ite E_hd g_hd ns_hd ls_hd ls_tl) => [[[[E_ite g_ite] cs_ite] ls_ite] Hite] .
     move : (IH _ _ _ _ _ Hrec) => HEEtl .
@@ -519,15 +549,12 @@ Lemma mk_env_shl_int_sat E g ls n E' g' cs lrs :
   newer_than_lits g ls ->
   interp_cnf E' cs .
 Proof .
-  elim : n E' g' cs lrs => [|n IH] E' g' cs lrs .
-  - rewrite /mk_env_shl_int /= .
-    by case => <- _ <- _ .
-  - rewrite /mk_env_shl_int /= -/mk_env_shl_int .
-    dcase (mk_env_shl_int E g ls n) => [[[[E_m g_m] cs_m] ls_m] Hint] .
-    case => <- _ <- _ .
-    rewrite interp_cnf_catrev => Hgls .
-    move : (IH _ _ _ _ Hint Hgls) .
-    by t_auto_newer .
+  move: E' g' cs lrs. eapply mk_env_shl_int_ind.
+  - clear n. move=> n Hn E' g' cs lrs [] ? ? ? ?; subst => /=. done.
+  - clear n. move=> n [] p Hn //=. move=> _ IH E_m g_m cs_m ls_m Henv.
+    move=> E1 g1 cs1 ls1 [] ? ? ? ?; subst. move=> E' g' cs lrs [] ? ? ? ?; subst.
+    move=> Hgls. rewrite interp_cnf_catrev.
+    by rewrite (IH _ _ _ _ Henv Hgls) /=.
 Qed .
 
 Lemma mk_env_shl_rec_sat E g ls ns i E' g' cs lrs :
@@ -540,7 +567,7 @@ Proof .
   - rewrite /mk_env_shl_rec /= .
     by case => <- _ <- _ .
   - rewrite /mk_env_shl_rec /= -/mk_env_shl_rec .
-    dcase (mk_env_shl_rec E g ls ns_tl (2*i)) => [[[[E_tl g_tl] cs_tl] ls_tl] Hrec] .
+    dcase (mk_env_shl_rec E g ls ns_tl (i*2)) => [[[[E_tl g_tl] cs_tl] ls_tl] Hrec] .
     dcase (mk_env_shl_int E_tl g_tl ls_tl i) => [[[[E_hd g_hd] cs_hd] ls_hd] Hint] .
     dcase (mk_env_ite E_hd g_hd ns_hd ls_hd ls_tl) => [[[[E_ite g_ite] cs_ite] ls_ite] Hite] .
     move => Htmp Hgtt Hgls /andP [Hgnshd Hgnstl] .
